# Question 1

$(\lambda xyz \mid x(y(yyz))) \space (\lambda x \mid x) \space (\lambda x \mid x(qq)) \space a$

Applicative order
$(\lambda xyz \mid x(y(yyz))) \space (\lambda x \mid x) \space (\lambda x \mid x(qq)) \space a$
$(\lambda yz \mid (\lambda x \mid x) (y(yyz))) \space (\lambda x \mid x(qq)) \space a$
$(\lambda z \mid (\lambda x \mid x) ((\lambda x \mid x(qq))((\lambda x \mid x(qq))(\lambda x \mid x(qq))z))) \space a$
$(\lambda x \mid x) ((\lambda x \mid x(qq))((\lambda x \mid x(qq))(\lambda x \mid x(qq))a))$
$((\lambda x \mid x(qq))((\lambda x \mid x(qq))(\lambda x \mid x(qq))a))$
$((\lambda x \mid x(qq))((\lambda x \mid x(qq))(a(qq)))$
$((\lambda x \mid x(qq))((a(qq))(qq))$
$((\lambda x \mid x(qq))((a(qq))(qq))$
$((a(qq))(qq))(qq)$














