1. 
	   <br>To show that $\vec{v} \sim \vec{v'}$ is an equivalence relation we need to show that it follows the 3 properties of an equivalence relation
	
	Reflexive Property:
		$T(\vec{v}) = T(\vec{v'}) \implies \vec{v} = \vec{v'}$
	Symmetric Property:
		$T(\vec{v}) = T(\vec{v'}) \implies \vec{v} = \vec{v'} \implies \vec{v'} = \vec{v}$
	Transitive Property
		$T(\vec{v}) = T(\vec{v'})$
		$T(\vec{v'}) = T(\vec{v''})$
		$T(\vec{v}) = T(\vec{v'}) = T(\vec{v''}) \implies T(\vec{v}) = T(\vec{v''})$
	$QED$

2. <br>(a)
	
	We need to show that $\vec{u} \sim \vec{v} \implies f(\vec{u}) = f(\vec{v}) \quad \forall \; \vec{u}, \vec{v} \in \mathbb{C}^3/\sim$
	However this is not true for the example relation given in the question
	
	$\vec{u} = (-i, i + 1, i -1), \quad \vec{v} = (0,0,0)$ 
	$\vec{u} \sim \vec{v}$
	$f(\vec{u}) = (-i, i + 1)$
	$f(\vec{v}) = (0,0)$
	$(-i, i + 1) \neq (0,0)$
	
	$\therefore \; f$ is not well defined over $\mathbb{C}^3/\sim$
	
	(b)
	
	
