
# Problem 1.
$\frac{d}{dx} \cot^{-1}(\sinh(x)) = \frac{-1}{1+ (\sinh(x))^2} \cosh(x)$
$\Rightarrow \frac{-\cosh(x)}{1+ \sinh^2(x)}$
Using the identity $\cosh(x)^2 - \sinh(x)^2 = 1$ this simplifies to
$\Rightarrow \frac{-\cosh(x)}{\cosh^2(x)}$
$\Rightarrow \frac{-1}{\cosh(x)}$
$\Rightarrow -\operatorname{sech}(x)$
# Problem 2.
The proposed solution to the differential equation $\theta = A\cosh(\omega t) + B\sinh(\omega t)$ has derivatives
$\theta' = A\omega \sinh(\omega t) + B\omega \cosh(\omega t) \quad and \quad \theta'' = A\omega^2 \cosh(\omega t) + B\omega^2 \sinh(\omega t)$
Substituting $\theta \text{ and } \theta''$ into the differential equation gives
$\Rightarrow (A\omega^2 \cosh(\omega t) + B\omega^2 \sinh(\omega t)) = \omega^2 (A\cosh(\omega t) + B\sinh(\omega t))$
$\Rightarrow \omega^2(A\cosh(\omega t) + B\sinh(\omega t)) = \omega^2 (A\cosh(\omega t) + B\sinh(\omega t))$
$\Rightarrow 1=1$
$\Rightarrow LHS=RHS$
$\therefore \; \theta = A\cosh(\omega t) + B\sinh(\omega t)$ is a solution to the differential equation

# Problem 3.
The proposed solution to the differential equation $y= k\cosh(\frac{x}{k})$ has derivatives
$y' = \sinh(\frac x k )\quad and \quad y'' = \frac 1 k \cosh(\frac x k)$
Substituting $y' \; and \; y''$ into the differential equation gives
$\Rightarrow k^2 \left( \frac  {\cosh(\frac x k)}{k} \right) ^2 - \left( \sinh(\frac x k )\right) ^2 = 1$
$\Rightarrow \cosh^2(\frac x k) - \sinh^2(\frac x k) = 1$
Using the identity $\cosh^2(x) - \sinh^2(x) = 1$ the equation becomes
$\Rightarrow 1=1$
$\Rightarrow LHS=RHS$
$\therefore \; y = \cosh(\frac x k)$ is a solution to the differential equation
