1. 
	$\Rightarrow \frac{(\overline{2+22-5})(\overline{9+6})}{\overline{4}}$
	$\Rightarrow \frac{(\overline{19})(\overline{15})}{\overline{4}}$
	$\Rightarrow \frac{(\overline{8})(\overline{4})}{\overline{4}}$
	$\Rightarrow \overline{8}$
		 <div style="page-break-after: always; visibility: hidden">\pagebreak</div>
2. 
	(a)
	$x = \frac{\overline{5}}{\overline{3}}$
	$x = \frac{\overline{18}}{\overline{3}}$
	$x = \overline{\frac{18}{3}}$
	$x = \overline{6}$
	(b)
	$x = \sqrt{\overline{0}}$
	$x = \pm \; \overline{0}$
	$x = \overline{0}$
	(c)
	$x = \sqrt{\overline{1}}$
	$x = \sqrt{\overline{144}}$
	$x = \pm \overline{12}$
	$x = \overline{-1}, \overline{1}$
	(d)
	$x = \sqrt{\overline{-1}}$
	$x = \sqrt{\overline{25}}$
	$x = \pm \overline{5}$
	$x = \overline{-5}, \overline{5}$
	<div style="page-break-after: always; visibility: hidden">\pagebreak</div>
3. 
	(a)
	DNE
	(b)
	$x = \sqrt{\overline{0}}$
	$x = \sqrt{\overline{36}}$
	$x = \overline{6}$
	(c)
	$x = \sqrt{\overline{1}} = \sqrt{\overline{25}}$
	$x = \pm \overline{1}, \pm \overline{5}$
	$x = \overline{1},  \overline{5},  \overline{7},  \overline{11}$
	(d)
	$x = \sqrt{\overline{-1}}$
	DNE
		 <div style="page-break-after: always; visibility: hidden">\pagebreak</div>
4. 
	(a)
	$\exists (\overline{1},\overline{0}) \in \mathbb{F}^2_3 \text{ Such That } (a,b)(\overline{1},\overline{0}) = (a,b) \quad \forall (a,b) \in  \mathbb{F}^2_3$
	$\Rightarrow (a\overline{1} - b\overline{0}, a\overline{0} + b\overline{1}) = (a,b)$
	$\Rightarrow (a,b) = (a,b)$

	$\exists (\overline{0},\overline{0}) \in \mathbb{F}^2_3 \text{ Such That } (a,b) + (\overline{0},\overline{0}) = (a,b) \quad \forall (a,b) \in  \mathbb{F}^2_3$
	$\Rightarrow (a+\overline{0},b+\overline{0}) = (a,b)$
	$\Rightarrow (a,b) =(a,b)$

	The multiplicative inverse states that $(a,b)(a,b)^{-1} = (\overline{1},\overline{0}) \quad \forall \in \mathbb{F}^2_3 \text{ Such That }(a,b)^{-1} \neq (\overline{0},\overline{0})$

	$\Rightarrow (a,b)(\frac{a}{a^2+b^2}, \frac{-b}{a^2+b^2}) = (\overline{1},\overline{0}) \quad a^2+b^2 \neq 0$
	$\Rightarrow (\frac{a^2}{a^2+b^2} - \frac{-b^2}{a^2+b^2}, \frac{-ab}{a^2+b^2} - \frac{ab}{a^2+b^2}) = (\overline{1},\overline{0})$
	$\Rightarrow (\frac{a^2 + b^2}{a^2+b^2}, \frac{ab-ab}{a^2+b^2}) = (\overline{1},\overline{0})$
	$\Rightarrow (\overline{1},\overline{0})  = (\overline{1},\overline{0}) \quad \forall (a,b) \text{ Such That } a^2+b^2 \neq 0$
	
	To check that $a^2 + b^2 \neq 0 \quad \forall (a,b) \in \mathbb{F}^2_3 \text{ except } (0,0)$ we need to check every element of  $\mathbb{F}_3$. $\quad \mathbb{F}_3$ consists of the elements $\{-1, 0, 1\}$ 
	$(-1)^2 = 1$
	$1^2 = 1$
	$0^2 = 0$
	Therefore we have to check every combination of $a,b \in \{0,1\}$ against the equation  $a + b\neq 0$
	Case 1: $a,b = 1$
	$1+1 \neq 0$
	$2 \neq 0$
	Case 2: $a = 1, b = 0$
	$1+0 \neq 0$
	$1 \neq 0$
	Case 3: a = 0, b = 1
	$0+1\neq 0$
	$1 \neq 0$
	Case 4 : $a,b = 0$
	$0+0 \neq 0$
	$0 \neq 0$
	This is false
	$\therefore$ the restriction $a^2 + b^2 \neq 0$ can be simplified to just $(a,b) \neq (0,0)$ which is the original stipulation of the axiom,  making the axiom valid in $\mathbb{F}^2_3$
	 
	
	The Additive inverse states that $\exists -(a,b) \in \mathbb{F}^2_3 \text{ Such That } (a,b) + -(a,b) = (0,0)$
	$\Rightarrow (a,b) + (-a,-b) = (0,0)$
	$\Rightarrow (a-a, b-b) = (0,0)$
	$\Rightarrow (0,0) = (0,0)$
	
	With both identities and both inverses proved we can conclude that $\mathbb{F}^2_3$ Must be a field
	
	(b)
	$\exists (\overline{1},\overline{0}) \in \mathbb{F}^2_5 \text{ Such That } (a,b)(\overline{1},\overline{0}) = (a,b) \quad \forall (a,b) \in  \mathbb{F}^2_5$
	$\Rightarrow (a\overline{1} - b\overline{0}, a\overline{0} + b\overline{1}) = (a,b)$
	$\Rightarrow (a,b) = (a,b)$

	$\exists (\overline{0},\overline{0}) \in \mathbb{F}^2_5 \text{ Such That } (a,b) + (\overline{0},\overline{0}) = (a,b) \quad \forall (a,b) \in  \mathbb{F}^2_5$
	$\Rightarrow (a+\overline{0},b+\overline{0}) = (a,b)$
	$\Rightarrow (a,b) =(a,b)$

	The multiplicative inverse states that $(a,b)(a,b)^{-1} = (\overline{1},\overline{0}) \quad \forall \in \mathbb{F}^2_5 \text{ Such That }(a,b)^{-1} \neq (\overline{0},\overline{0})$

	$\Rightarrow (a,b)(\frac{a}{a^2+b^2}, \frac{-b}{a^2+b^2}) = (\overline{1},\overline{0}) \quad a^2+b^2 \neq (\overline{0}, \overline{0})$
	$\Rightarrow (\frac{a^2}{a^2+b^2} - \frac{-b^2}{a^2+b^2}, \frac{-ab}{a^2+b^2} - \frac{ab}{a^2+b^2}) = (\overline{1},\overline{0})$
	$\Rightarrow (\frac{a^2 + b^2}{a^2+b^2}, \frac{ab-ab}{a^2+b^2}) = (\overline{1},\overline{0})$
	$\Rightarrow (\overline{1},\overline{0})  = (\overline{1},\overline{0}) \quad \forall (a,b) \text{ Such That } a^2+b^2 \neq (\overline{0}, \overline{0})$
	We are trying to prove $\mathbb{F}^2_5$ is a field, we propose the following counter example to the axiom of multiplicative inverse

	Let $A = (\overline{2},\overline{4})$
	If $\overline{2^2} +  \overline{4^2} = \overline{0}$ then $A$ does not have a multiplicative inverse as proved above
	$\Rightarrow \overline{4} + \overline{16} \stackrel{?}{=} \overline{0}$
	$\Rightarrow \overline{4+16} \stackrel{?}{=} \overline{0}$
	$\Rightarrow \overline{20} \stackrel{?}{=} \overline{0}$
	$\Rightarrow \overline{0} = \overline{0}$ 
	$\therefore A$ Does not have a multiplicative inverse and $A$ is not the additive identity which violates the axiom of multiplicative inverse making $\mathbb{F}^2_3$ not a field
	<div style="page-break-after: always; visibility: hidden">\pagebreak</div>
5. 
	(a)
	$a \odot (b \oplus c) = (a \odot b) \oplus (a \odot c)$
	$a + (b \oplus c) = (a + b) \oplus (a + c)$
	
	Case 1:  $b<c$
	$a + (b) = (a+b)$
	$a+b = a+b$
	
	Case 2: $c \le b$
	$a + (c) = (a+c)$
	$a+c = a+c$
	
	It works for both cases which means it works for all $a,b,c \in F$ so it must be valid
	(b)
	$\exists 0 \in F \text{ Such That } a \odot 0 = a$
	$\Rightarrow a+0 = a$
	$\Rightarrow a=a$
	(c)
	The multiplicative inverse of 2 is defined to be $2 \odot 2^{-1} = 0$
	$\Rightarrow 2 + 2^{-1} = 0$
	$\Rightarrow 2^{-1} = -2$
	$\therefore$ the original equation becomes $5 \odot -2$
	$\Rightarrow 5 \odot -2 = 3$
	(d)
	The axiom of additive identity states that there is exactly one additive identity in a field however for $F$ there are infinity many additive identities, for example
	$-3 \oplus 1 = -3$
	$5 \oplus 6 = 5$
	$\therefore$ $6 \text{ and } 1$ are both additive identities for $F$ making it not a field
	<div style="page-break-after: always; visibility: hidden">\pagebreak</div>
6. 
	(a)
	$\exists -1 \in F \text{ Such That } a \oplus -1 = a$
	in $F \; -1$ is the largest number therefore when you take the minimum of any number $a$ and $-1$ it will always return a as $a \le -1 \quad \forall a \in F$ 
	(b)
	There is only one pair of numbers $a,b \in F$ such that $a \oplus b = -1$
	$a,b = -1$
	$\Rightarrow -1 \oplus -1 = -1$
	For any $a \text{ or } b < -1$ this would not work as $\oplus$ would always just return $a \text{ or } b$ not $-1$
	<div style="page-break-after: always; visibility: hidden">\pagebreak</div>
7. 
	(a)
	$\exists \; 2x \in \mathbb{F} \text{ Such That } x + x = 2x$
	By the Distributive Property
	$\Rightarrow x(1+1) = 2x$
	By the cancellation law for multiplication
	$\Rightarrow (1+1) = 2$
	$\Rightarrow 1 + 1 = 2$
	$\Rightarrow 2=2$
	QED
	
	(b)
	$2x = 2y$
	Multiplying both sides by $2^{-1}$
	$\Rightarrow (22^{-1})x = (22^{-1})y$
	By the property of multiplicative inverse
	$\Rightarrow 1x = 1y$ where $1$ is the multiplicative identity or "Unity" for any field $F$ 
	By the axiom of multiplicative identity $1a = a$
	$\Rightarrow x=y$


	The only Field this does not work for is $F_2$ as $2x=2y$ simplifies to $\overline{0} = \overline{0}$ which is always true no matter what $x,y$ you choose 
	eg. you could choose $x=\overline{0}, y = \overline{1}$
	$\Rightarrow 2(\overline{0}) = 2(\overline{1})$
	$\Rightarrow \overline{0} = \overline{2}$
	$\Rightarrow \overline{0} = \overline{0}$
	$\therefore$ $2x = 2y$ but $x \neq y$ which means this statement is false