# Question 3

(a)

$p(x).(u+v) = (a_0 + a_1(2)^1 + a_2(2)^2 + \dots + a_n(2)^n)(u+v)$
Since both elements are now just real numbers we can use distributivity
$p(2) = a_0 + a_1(2)^1 + a_2(2)^2 + \dots + a_n(2)^n$
$p(x).(u+v) = (p(2))u + (p(2))v$
$p(x).(u+v) = (p(x)).u + (p(x)).v$

(b)

Assume for contradiction there is such a $T$, Let $T(1) = w$

$T(p(x).1) = p(x).T(1) = p(x).w = p(3)w$
$T(p(x).1) = T(p(2)1) = p(2)T(1) = p(2)w$
$p(3)w = p(2)w$
$p(3) = p(2)$
this is a contradiction as for example it is not true for $p(x) = x$