# Question 4

(a)

$\operatorname{det}(-5A^2B^3A^T) = \operatorname{det}(-5)\operatorname{det}(A^2)\operatorname{det}(B^3)\operatorname{det}(A^T) \neq 0$
$\operatorname{det}(-5A^2B^3A^T) = (-5)^n\operatorname{det}(A)^2\operatorname{det}(B)^3\operatorname{det}(A) \neq 0$
$\operatorname{det}(-5A^2B^3A^T) = (-5)^n\operatorname{det}(A)^3\operatorname{det}(B)^3 \neq 0$
$\therefore \; \operatorname{det}(A) \neq 0\text{ and } \operatorname{det}(B) \neq 0 \implies$ invertible

(b)

$\operatorname{det}(2AB^{-1}A^TB^2) = 2^3\operatorname{det}(A)\operatorname{det}(B)^{-1}\operatorname{det}(A)\operatorname{det}(B)^2$
$\operatorname{det}(2AB^{-1}A^TB^2) = 8(-1)2^{-1}(-1)(4)$
$\operatorname{det}(2AB^{-1}A^TB^2) = 16$

(c)

$\operatorname{det}(A^T) = \operatorname{det}(A)$
$\operatorname{det}(-A) = \operatorname{det}(A)$
$\operatorname{det}(-A) = \operatorname{det}(-I_7)\operatorname{det}(A)$
$\operatorname{det}(-A) = (-1)^7 \operatorname{det}(A)$
$\operatorname{det}(-A) = -\operatorname{det}(A) = \operatorname{det}(A)$
$\operatorname{det}(A) = -\operatorname{det}(A) \implies \operatorname{det}(A) = 0 \implies$ not invertible