# Question 6

(a)

$$[T(x^4)]_{\beta'} = \begin{pmatrix} 2\\1\\1\\0 \end{pmatrix}$$ 
$$[T(x^3)]_{\beta'} = \begin{pmatrix} -2\\-1\\-1\\0 \end{pmatrix}$$ 
$$[T(x^2)]_{\beta'} = \begin{pmatrix} -1\\-2\\-2\\1 \end{pmatrix}$$ 
$$[T(x)]_{\beta'} = \begin{pmatrix} 0\\3\\0\\1 \end{pmatrix}$$ 
$$[T(1)]_{\beta'} = \begin{pmatrix} 1\\-1\\-1\\1 \end{pmatrix}$$ 
$$[T]_{\beta' \leftarrow \beta} = \begin{pmatrix} 2 & -2 & -1& 0 & 1\\1 & -1 & -2 & 3 & -1\\1 & -1 & -2 & 0 & -1\\0 & 0 & 1 & 1 & 1 \end{pmatrix} $$
(b)

$$[(x^4 - x^3 + x)]_{\beta} = \begin{pmatrix} 1\\-1\\0\\1\\0 \end{pmatrix}$$ 
$$[T(x^4 - x^3 + x)]_{\beta'} = \begin{pmatrix} 4\\5\\2\\1\ \end{pmatrix}$$ 
$$[T(x^4 - x^3 + x)]_{\beta'} = \begin{pmatrix} 2 & -2 & -1& 0 & 1\\1 & -1 & -2 & 3 & -1\\1 & -1 & -2 & 0 & -1\\0 & 0 & 1 & 1 & 1 \end{pmatrix}\begin{pmatrix} 1\\-1\\0\\1\\0 \end{pmatrix} = \begin{pmatrix} 4\\5\\2\\1 \end{pmatrix}$$

They both get the same answer so the formula holds